src/inductive/inductive_graph_theory_mkGraph.v
@@ -29,17 +29,120 @@ Require Import GraphVerification.src.util.util.
 (* Stating and proving Lemmas and Theorems about IG_mkGraph and helper functions *)
 
 
-Lemma _insNode_any_ins_node : forall (A B : Type) (node : LNode A) (ig : IG A B) (x : LNode A),
-    In node (IG_labNodes (_insNode node ig)). 
 
+
+
+
+
+
+(* Here, one may consider using IG_match as a probing tool instead of IG_labNodes *)
+(* Lemma IG_and_adds_node : forall (A B : Type) (c : Context A B) (ig : IG A B),
+    let '(_, node, label, _) := c in
+    _key_In_IG node ig
+        -> forall x, 
+        In x (IG_labNodes (IG_and c ig)) <-> In x ([(node, label)] ++ IG_labNodes ig).
 Proof.
-    intros. simpl.
-    destruct node.
-    pose proof (IG_and_adds_node _ B (nil, n, a, nil)).
+    intros.
+    destruct_context c.
+    intros. unfold _key_In_IG in H. unfold not in H.
+    unfold IG_and.
+    destruct (NatMap.mem node ig) eqn:cond.
+    - exfalso. apply H. clear H.
+        apply MFacts.mem_in_iff in cond. firstorder.
+        destruct_context' x. exists label'.
+        apply _In_labNodes_is_some_MapsTo.
+        firstorder.
+    - clear H. rewrite _updAdj_addSucc_does_not_change_IG_labNodes.
+        rewrite _updAdj_addPred_does_not_change_IG_labNodes.
+        rewrite _In_labNodes_is_some_MapsTo.
+        simpl.
+        (* This allows for rewriting within an exists *)
+        setoid_rewrite MFacts.add_mapsto_iff.
+        rewrite _In_labNodes_is_some_MapsTo.
+        apply MFacts.not_mem_in_iff in cond.
+        destruct x. simpl.
+        firstorder. 
+        + inversion H1. subst.  firstorder.
+        + inversion H0. subst. exists froms, tos. firstorder.
+        + bdestruct (node =? n).
+            -- subst. firstorder.
+            -- firstorder.
+Qed. *)
+
+
+Lemma IG_and_adds_node : forall (A B : Type) (c : Context A B) (ig : IG A B) (x : LNode A),
+    In x (IG_labNodes (IG_and c ig))
+        <-> let '(_, node, label, _) := c in (x = (node, label) /\ ~_key_In_IG (fst x) ig) \/ In x (IG_labNodes ig).
+Proof.
+    intros.
+    destruct_context c.
+
+    unfold _key_In_IG.
+    unfold IG_and.
+    destruct (NatMap.mem node ig) eqn:cond.
+    - split; intros.
+        + firstorder.
+        + destruct H.
+            -- destruct H. unfold not in H0. exfalso. apply H0. destruct x as [xn xl]. inversion H. subst.
+                apply MFacts.mem_in_iff in cond.
+                apply -> NatMap_In_exists_MapsTo_iff in cond. destruct cond. destruct_context' x.
+                exists label'.
+                apply _In_labNodes_is_some_MapsTo. firstorder.
+            -- assumption.
+    - rewrite _updAdj_addSucc_does_not_change_IG_labNodes.
+        rewrite _updAdj_addPred_does_not_change_IG_labNodes.
+        rewrite _In_labNodes_is_some_MapsTo. destruct x as [xn xl]. 
+        simpl.
+
+        (* This allows for rewriting within an exists *)
+        setoid_rewrite MFacts.add_mapsto_iff.
+        rewrite _In_labNodes_is_some_MapsTo.
+        apply MFacts.not_mem_in_iff in cond.
+        simpl.
+        firstorder. 
+        + inversion H1. subst. left. split.
+            -- reflexivity.
+
+            -- unfold not. intros. destruct H0.
+                apply _In_labNodes_is_some_MapsTo in H0.
+                firstorder.
+        + inversion H0. subst. exists froms, tos. firstorder.
+        + bdestruct (node =? xn).
+            -- subst. firstorder.
+            -- firstorder.
+Qed.
+
+
+
+
+
+
+
+
+
+
+
+
+(* Lemma _insNode_any_ins_node : forall (A B : Type) (node : LNode A) (ig : IG A B) (x : LNode A),
+    _key_In_IG (fst node) ig
+        -> In x (IG_labNodes (_insNode node ig)) <-> In x (node :: IG_labNodes ig).
+Proof.
+    intros.
     unfold _insNode.
-    rewrite H.
-    simpl.
-    reflexivity.
+    destruct node. intros.
+    pose proof (IG_and_adds_node _ B (nil, n, a, nil)).
+    apply H0.
+    assumption.
+Qed. *)
+
+Lemma _insNode_any_ins_node : forall (A B : Type) (node : LNode A) (ig : IG A B) (x : LNode A),
+    In x (IG_labNodes (_insNode node ig)) <-> (x = node /\ ~_key_In_IG (fst x) ig ) \/ In x (IG_labNodes ig).
+Proof.
+    intros.
+    unfold _insNode.
+    destruct node. intros.
+    pose proof (IG_and_adds_node _ B (nil, n, a, nil)).
+    apply H.
 Qed.
 
 
@@ -50,13 +153,12 @@ Lemma _mem_different_insNodes : forall (A B : Type) (n : Node) (a : A) (nodes : 
 Proof.
     intros. induction nodes.
     - simpl. reflexivity.
-    - simpl. destruct a0. assert (~ InA (fun x y : NatSet.Node * A => fst x = fst y) (n, a) nodes). {
-        firstorder.
+    - simpl. destruct a0. assert (~ InA (fun x y => fst x = fst y) (n, a) nodes). {
+            firstorder.
         } apply IHnodes in H0.
         assert (n <> n0). {
-        firstorder.
+            firstorder.
         }
-        
         destruct (NatMap.mem n ig) eqn:HH.
         + apply MFacts.mem_in_iff. apply MFacts.mem_in_iff in H0. simpl. destruct (NatMap.mem n0 (_insNodes nodes ig)).
         -- assumption.
@@ -70,38 +172,145 @@ Qed.
 
 
 
-Lemma _insNodes_any_ins_all_nodes : forall (A B : Type) (nodes : list (LNode A)) (ig : IG A B) (x : LNode A),
-    NoDupA (fun x y => fst x = fst y) nodes ->
-    In x (IG_labNodes (_insNodes nodes ig)) <-> In x (filter (fun '(n, _) => negb (NatMap.mem n ig)) nodes ++ IG_labNodes ig).
-Proof.
-    intros. induction nodes.
-        - simpl. reflexivity.
-        - simpl. inversion H. apply IHnodes in H3. rewrite _insNode_any_ins_node. destruct a. simpl.
-        apply (_mem_different_insNodes _ B _ _ _ ig) in H2.
-        rewrite H2.
-        destruct (NatMap.mem n ig) eqn:HH.
 
-        + simpl. rewrite H3. reflexivity.
-        + simpl. rewrite H3. reflexivity.
+(* Lemma _insNodes_any_ins_all_nodes : forall (A B : Type) (nodes : list (LNode A)) (ig : IG A B) (x : LNode A),
+    NoDupA (fun x y => fst x = fst y) nodes
+        -> In x (IG_labNodes (_insNodes nodes ig)) <-> In x (filter (fun '(n, _) => _key_In_IGb n ig) nodes ++ IG_labNodes ig).
+Proof.
+    intros. induction nodes; simpl.
+    - reflexivity.
+    - inversion H. specialize (IHnodes H3). subst. clear H.
+        destruct a as [an al].
+        apply (_mem_different_insNodes _ B _ _ _ ig) in H2.
+    
+        destruct (NatMap.mem an ig) eqn:HH.
+            + simpl. rewrite H2.
+                rewrite _key_In_IGb_is_mem.                
+                rewrite HH.
+                apply IHnodes.
+            + rewrite _insNode_any_ins_node.
+                -- simpl.
+                    rewrite _key_In_IGb_is_mem.
+                    rewrite HH.
+                    simpl. rewrite IHnodes. reflexivity.
+                -- simpl. unfold _key_In_IG. unfold not. intros.
+                    destruct H.
+                    apply _In_labNodes_is_some_MapsTo in H.
+                    apply MFacts.not_mem_in_iff in H2. unfold not in H2. apply H2. 
+                    rewrite NatMap_In_exists_MapsTo_iff.
+                    firstorder.
+Qed. *)
+
+Lemma _MapsTo_same_on_different_insNodes : forall (A B : Type) (n : Node) (a : A) (nodes : list (LNode A)) (ig : IG A B),
+    ~ InA (fun x y : NatSet.Node * A => fst x = fst y) (n, a) nodes
+        -> forall c, NatMap.MapsTo n c (_insNodes nodes ig) <-> NatMap.MapsTo n c ig.  
+Proof.
+    intros. induction nodes; simpl.
+    - reflexivity.
+    - destruct a0. assert (~ InA (fun x y => fst x = fst y) (n, a) nodes). {
+            firstorder.
+        } specialize (IHnodes H0).
+        assert (n0 <> n). {
+            firstorder.
+        }
+        unfold _insNode. unfold IG_and.
+        destruct (NatMap.mem n0 (_insNodes nodes ig)) eqn:split.
+        + apply IHnodes.
+        + simpl. rewrite MFacts.add_mapsto_iff. firstorder.
 Qed.
+        
+        
+
+
+Lemma _key_In_IG_same_on_different_insNodes : forall (A B : Type) (n : Node) (a : A) (nodes : list (LNode A)) (ig : IG A B),
+    ~ InA (fun x y : NatSet.Node * A => fst x = fst y) (n, a) nodes ->
+    ~_key_In_IG n (_insNodes nodes ig) <-> ~_key_In_IG n ig.
+Proof.
+    intros.
+    unfold _key_In_IG.
+    setoid_rewrite _In_labNodes_is_some_MapsTo.
+    simpl.
+    unfold not.
+    split; intros; apply H0; destruct H1; destruct_eMapsTo H1;
+    exists x, efroms, etos; eapply _MapsTo_same_on_different_insNodes in H; apply H; apply H1.
+Qed.
+
+
+
+
+
+Lemma _insNodes_any_ins_all_nodes : forall (A B : Type) (nodes : list (LNode A)) (ig : IG A B) (x : LNode A),
+    NoDupA (fun x y => fst x = fst y) nodes
+        -> In x (IG_labNodes (_insNodes nodes ig)) <-> (In x nodes /\ ~_key_In_IG (fst x) ig) \/ In x (IG_labNodes ig).
+Proof.
+    intros. induction nodes; simpl.
+    - firstorder.
+    - inversion H. subst. specialize (IHnodes H3). clear H. destruct a as [an al].
+        rewrite _insNode_any_ins_node. rewrite IHnodes. clear IHnodes. split; intros.
+        +
+        (* apply (_mem_different_insNodes A B _ _ _ ig) in H2. *)
+            destruct H.
+            -- destruct H. left.  destruct x as [xn xl]. inversion H. subst.
+                split.
+                ++ firstorder.
+                ++ eapply _key_In_IG_same_on_different_insNodes in H2.
+                    apply H2.
+                    apply H0. 
+                
+            -- firstorder.
+        + destruct H.
+            -- destruct H. destruct H.
+                ++ left. destruct x. inversion H. subst. split.
+                    --- reflexivity.
+                    --- eapply _key_In_IG_same_on_different_insNodes in H2.
+                        apply H2.
+                        apply H0.
+                ++ firstorder.
+            -- firstorder.
+Qed.
+                
+             
+
+
+
+
+
+
+
+
+
+
+
+
+
+
+
+
+
+
+
+
+
+
 
 
 Lemma _insEdge_does_not_add_node : forall (A B : Type) (edge : LEdge B) (ig : IG A B) (x : LNode A),
   In x (IG_labNodes (_insEdge edge ig)) <-> In x (IG_labNodes ig).
 Proof.
-    intros. unfold _insEdge. destruct edge as [[from to] label].
+    intros. unfold _insEdge. destruct_edge edge.
     destruct (IG_match from ig) eqn:HH.
-    destruct m as [[[[froms n] l] tos] | ].
-    - rewrite IG_and_adds_node. destruct (NatMap.mem from i) eqn:HHH.
+    destruct m.
+    - destruct_context c.
+        destruct (NatMap.mem from i) eqn:HHH.
         + exfalso. apply IG_match_returns_node in HH as HHHH. subst.
         apply  MFacts.mem_in_iff in HHH.
         
-        assert (exists c, NatMap.MapsTo n c i). {
+        assert (exists c, NatMap.MapsTo node c i). {
             firstorder.
         }
-        destruct H as [[[fromss node] toss] H].
+        destruct H as [[[fromss nodes] toss] H].
 
-        assert (In (n, node) (IG_labNodes i)). {
+        assert (In (node, nodes) (IG_labNodes i)). {
             apply _In_labNodes_is_some_MapsTo. firstorder.
         }
 
@@ -109,7 +318,19 @@ Proof.
         unfold not in HH. apply HH. firstorder.
 
 
-        + simpl. apply IG_match_returns_node in HH as HHHH. subst. apply (IG_match_just_removes_node _ _ _ _ _ _ _ _ _ x) in HH. rewrite HH. simpl. reflexivity.
+        +
+        pose proof (IG_and_adds_node _ _ (froms, from, label, (el, to) :: tos) i).
+        destruct_contextt (froms, from, label, (el, to) :: tos).
+
+        rewrite H.
+        --        simpl. apply IG_match_returns_node in HH as HHHH. subst. 
+        Check IG_match_just_removes_node.
+        apply (IG_match_just_removes_node _ _ _ _ _ _ x) in HH. rewrite HH. simpl. reflexivity.
+        
+        IG_and_adds_node.
+        
+        
+
     - reflexivity.
 Qed.
 
@@ -153,22 +374,26 @@ Proof.
             ++ destruct a. simpl. reflexivity.
 Qed.
 
+
+
+
+
 (* "big" statement: *)
 Theorem IG_mkGraph_any_ins_all_nodes : forall (A B : Type) (nodes : list (LNode A)) (edges : list (LEdge B)) (x : LNode A),
-    NoDupA (fun x y => fst x = fst y) nodes ->
-    In x (IG_labNodes (IG_mkGraph nodes edges)) <-> In x nodes.
+    NoDupA (fun x y => fst x = fst y) nodes
+        -> In x (IG_labNodes (IG_mkGraph nodes edges)) <-> In x nodes.
 Proof.
-    intros. unfold IG_mkGraph. rewrite _insEdges_does_not_add_nodes. rewrite _insNodes_any_ins_all_nodes.
-    - rewrite app_nil_r. simpl. rewrite _filter_identity. reflexivity.
-    - assumption.
+        intros. unfold IG_mkGraph. rewrite _insEdges_does_not_add_nodes. rewrite _insNodes_any_ins_all_nodes.
+        - rewrite app_nil_r. simpl. rewrite _filter_identity. reflexivity.
+        - assumption.
 Qed.
 
 Lemma _not_NatMap_Empty_is_empty_false : forall (A : Type) (m : NatMap.t A),
     not (NatMap.Empty m) <-> NatMap.is_empty m = false.
 Proof.
-    intros. unfold not. rewrite MFacts.is_empty_iff. destruct (NatMap.is_empty (elt:=A) m) eqn:cond.
-    - firstorder. congruence.
-    - firstorder. congruence.
+        intros. unfold not. rewrite MFacts.is_empty_iff. destruct (NatMap.is_empty (elt:=A) m) eqn:cond.
+        - firstorder. congruence.
+        - firstorder. congruence.
 Qed.
 
 Theorem  IG_non_empty_isEmpty_false : forall (A B : Type) (nodes : list (LNode A)) (edges : list (LEdge B)),
